floyd/base2.v
@@ -3,6 +3,7 @@ Require Export VST.floyd.typecheck_lemmas.
 Require Export VST.floyd.functional_base.
 Require Export VST.floyd.seplog_tactics.
 Require Export VST.floyd.const_only_eval.
+Require Export compcert.cfrontend.Ctypes.
 
 Fixpoint delete_id {A: Type} i (al: list (ident*A)) : option (A * list (ident*A)) :=
  match al with
