veric/semax_call.v
@@ -21,6 +21,107 @@ Require Import VST.veric.semax_lemmas.
 Require Import VST.veric.Clight_lemmas.
 
 Local Open Scope pred.
+
+Lemma age_later {A} {agA : ageable A}: forall {w w1 w2} (AGE: age w w1) (L: laterR w w2), w1=w2 \/ laterR w1 w2.
+Proof. intros. induction L.
++ unfold age in *. rewrite AGE in H. left; inv H; trivial.
++ right. destruct (IHL1 AGE); subst. apply L2. eapply t_trans; eassumption.
+Qed.
+
+Lemma tc_val_sem_cast':
+  forall {cs: compspecs} t2 e2 rho Delta,
+      @typecheck_environ Delta rho ->
+      @denote_tc_assert cs (@typecheck_expr cs Delta e2) rho
+     &&  @denote_tc_assert cs (@isCastResultType cs (typeof e2) t2  e2) rho 
+     |-- !! @tc_val t2 (force_val (sem_cast (typeof e2) t2 (eval_expr e2 rho))).
+Proof.
+intros.
+intro phi.
+intros [? ?].
+eapply expr_lemmas.tc_val_sem_cast; eauto.
+Qed.
+
+Lemma typecheck_expr_sound' {cs: compspecs} :
+  forall Delta rho e,
+    @typecheck_environ Delta rho ->
+    @tc_expr cs Delta e rho |-- !! @tc_val (typeof e) (eval_expr e rho).
+Proof.
+intros.
+intros ? ?.
+simpl.
+eapply expr_lemmas4.typecheck_expr_sound; eauto.
+Qed.
+
+Lemma tc_environ_make_args':
+ forall {CS: compspecs} argsig retsig bl rho Delta,
+   tc_environ Delta rho ->
+  tc_exprlist Delta (snd (split argsig)) bl rho
+  |-- !! tc_environ (funsig_tycontext (argsig, retsig)) (make_args (map fst argsig)
+         (eval_exprlist (snd (split argsig)) bl rho) rho).
+Proof.
+intros. rename H into H2.
+unfold tc_environ.
+simpl.
+unfold tc_exprlist.
+revert bl; induction argsig; destruct bl as [ | b bl]; simpl; intros; unfold_lift.
+* hnf; intros. clear H.
+  split3; hnf; intros; try (simpl in *; rewrite PTree.gempty in H; inv H).
+  rewrite PTree.gempty. split; intro. inv H. destruct H. inv H.
+* apply prop_derives; intros. inv H.
+* destruct a as [i ti]; simpl.
+  destruct (split argsig) eqn:?.
+  simpl.
+  unfold_lift; apply prop_derives; intros; inv H.
+* destruct a as [i ti]; simpl.
+  destruct (split argsig) eqn:?.
+  specialize (IHargsig bl).
+  simpl denote_tc_assert.
+  rewrite !denote_tc_assert_andp.
+  simpl andp.
+  unfold_lift.
+  apply derives_trans with
+   (denote_tc_assert (typecheck_expr Delta b) rho &&
+   denote_tc_assert (isCastResultType (typeof b) ti b) rho &&
+   (!! typecheck_environ (funsig_tycontext (argsig, retsig))
+                    (make_args (map fst argsig)
+                       (eval_exprlist l0 bl rho) rho))).
+  apply andp_derives; auto.
+  clear IHargsig.
+  simpl. unfold_lift.
+  normalize.
+  destruct H as [? [? ?]].
+  unfold typecheck_environ; simpl.
+  match goal with |- ?A |-- ?B => apply derives_trans with
+      (!! tc_val' ti (force_val (sem_cast (typeof b) ti (eval_expr b rho))) && A)
+  end.
+  + apply andp_right; auto.
+    clear - H2.
+    apply derives_trans with (!! (tc_val (typeof b) (eval_expr b rho)) &&
+     !! (tc_val ti (force_val (sem_cast (typeof b) ti (eval_expr b rho))))).
+    - apply andp_right.
+      eapply derives_trans; [ | eapply typecheck_expr_sound']; eauto.
+      apply andp_left1. apply derives_refl.
+      pose proof expr_lemmas.tc_val_sem_cast.
+      apply tc_val_sem_cast'; auto.
+    - apply andp_left2.
+      apply prop_derives.
+      unfold tc_val'.
+      intros; auto.
+  + normalize. rename H3 into H8.
+    hnf; intros. simpl.
+    split3; auto.
+    unfold typecheck_temp_environ; intros.
+    destruct (ident_eq i id).
+    - subst.
+      rewrite PTree.gss in H4. inv H4.
+      rewrite Map.gss.
+      eexists; split; eauto.
+    - rewrite Map.gso by auto.
+      apply (H id ty).
+      rewrite PTree.gso in H4 by auto.
+      simpl. auto.
+Qed.
+
 Section extensions.
 Context {CS: compspecs} {Espec: OracleKind}.
 
@@ -648,7 +749,7 @@ Lemma semax_call_typecheck_environ:
       (fn_return f)  (glob_types Delta) (glob_specs Delta) (annotations Delta))
      (mkEnviron (filter_genv psi) (make_venv ve') (make_tenv te')).
 Proof. assert (H1:= True).
- intros.
+ intros. 
  pose (rho3 := mkEnviron (filter_genv psi) (make_venv ve') (make_tenv te')).
 
 unfold typecheck_environ. repeat rewrite andb_true_iff.
@@ -1426,16 +1527,24 @@ forall (Delta : tycontext) (A : TypeTree)
  (TC3 : guard_environ Delta (current_function k) rho)
  (TC5 : retty = Tvoid -> ret = None)
  (H : closed_wrt_modvars (Scall ret a bl) F0)
- (HR : RA_normal R =
+
+(* LENB: replace eqality with entailment -- notice the |>
+  (HR : RA_normal R =
      (fun rho0 : environ =>
       EX  old : val,
-      substopt ret old F rho0 * maybe_retval (Q ts x) retty ret rho0))
+      substopt ret old F rho0 * maybe_retval (Q ts x) retty ret rho0))*)
+(HR: ( ( |> ALL rho' : environ ,
+       !((EX old:val, substopt ret old F rho' * maybe_retval (Q ts x) retty ret rho') >=> (RA_normal R rho') ))) (m_phi jm))
+
  (HGG:  genv_cenv psi = cenv_cs)
  (H0 : rho = construct_rho (filter_genv psi) vx tx)
  (H3 : eval_expr a rho = Vptr b Ptrofs.zero)
  (H4 : (funassert Delta rho) (m_phi jm))
- (H1 : (rguard Espec psi Delta
+
+  (*LENB: now with a |> here*)
+ (H1 : (|> rguard Espec psi Delta
         (frame_ret_assert R F0) k) (level (m_phi jm)))
+
  (H11 : forall vl : environ, (!|>(Q' ts x vl <=> Q ts x vl)) (m_phi jm))
  (H14 : (|>(F0 rho * F rho *
           P ts x
@@ -1596,17 +1705,37 @@ specialize (H15 m' (le_refl _) _ (necR_refl _) H8).
 pose (tx' := match ret,ret0 with
                    | Some id, Some v => PTree.set id v tx
                    | _, _ => tx
-                   end).
-
+                   end). 
+assert (LAT: laterM (level (m_phi jm)) (level jm')). { simpl; apply laterR_level'. constructor. apply age_jm_phi. apply Hage. }
+specialize (H1 _ LAT).
 specialize (H1 EK_normal None tx' vx (m_phi m')).
+assert (LATER: laterM (m_phi jm) (m_phi jm')). { clear - Hage. apply age_laterR. apply age1_juicy_mem_Some in Hage; trivial. }
+specialize (HR (m_phi jm') LATER (construct_rho (filter_genv psi) vx tx')); hnf in HR. 
 spec H1.
-{ clear - Hage H9.
-  change (level jm >= level m')%nat.
-  apply age_level in Hage. omega.
+{ clear - Hage H9. rewrite <- level_juice_level_phi. omega.
+  (*change (level jm >= level m')%nat.
+  apply age_level in Hage. omega.*)
 }
 rewrite proj_frame_ret_assert in H1.
-simpl proj_ret_assert in H1.
-rewrite HR in H1; clear R HR.
+simpl proj_ret_assert in H1. hnf in H1. 
+
+(*rewrite HR in H1; clear R HR.*)
+assert (H1' : forall a' : rmap,
+     necR (m_phi m') a' ->
+     (!! guard_environ Delta (current_function k) (construct_rho (filter_genv psi) vx tx') &&
+      seplog.sepcon (fun rho0 => EX old:val, substopt ret old F rho0 * maybe_retval (Q ts x) retty ret rho0) F0 (construct_rho (filter_genv psi) vx tx') &&
+      funassert Delta (construct_rho (filter_genv psi) vx tx')) a' ->
+     (assert_safe Espec psi vx tx' (exit_cont EK_normal None k) (construct_rho (filter_genv psi) vx tx')) a').
+{ intros a' NEC Ha'. apply (H1 _ NEC); clear H1.
+  destruct Ha' as [HX HY].
+  split; trivial. clear HY. destruct HX as [HA HB]. split; trivial. clear HA.
+  destruct HB as [a1 [a2 [J [A1 A2]]]]. exists a1, a2; split; [trivial | split ;[| trivial]].
+  destruct (nec_join4 _ _ _ _ J NEC) as [a1' [a2' [J' [NA1 NA2]]]].
+  eapply HR; try eassumption.
+  apply join_level in J'; destruct J' as [J' _]; rewrite J'.
+  rewrite <- 2 level_juice_level_phi. destruct H6 as [? [? ?]]; subst. omega. } 
+clear H1; rename H1' into H1. clear R HR.
+
 simpl exit_cont in H1.
 do 3 red in H5.
 specialize (H1 _ (necR_refl _)).
@@ -1975,7 +2104,54 @@ destruct (type_eq retty Tvoid).
 destruct H6 as (?&?&?).
 subst n'.
 rewrite level_juice_level_phi.
-destruct ret; destruct ret0; apply assert_safe_jsafe; auto.
+destruct ret; destruct ret0; apply assert_safe_jsafe; auto. 
+Qed.
+
+Lemma semax_call_external':
+forall (Delta : tycontext) (A : TypeTree)
+  (P Q Q' : forall ts, dependent_type_functor_rec ts (AssertTT A) mpred)
+  (ts: list Type) (x : dependent_type_functor_rec ts A mpred)
+  (F : environ -> pred rmap) (F0 : assert)
+  (ret : option ident) (params : list (ident * type)) (retty : type) cc
+  (a : expr) (bl : list expr) (R : ret_assert) (psi : genv) (vx : env)
+  (tx : temp_env) (k : cont) (rho : environ) (ora : OK_ty) (jm : juicy_mem)
+  (b : block)
+ (TC0 : Cop.classify_fun (typeof a) =
+      Cop.fun_case_f (type_of_params params) retty cc)
+ (TCret : tc_fn_return Delta ret retty)
+ (TC1 : (|> tc_expr Delta a rho) (m_phi jm))
+ (TC2 : (|> tc_exprlist Delta (map snd params) bl rho) (m_phi jm))
+ (TC3 : guard_environ Delta (current_function k) rho)
+ (TC5 : retty = Tvoid -> ret = None)
+ (H : closed_wrt_modvars (Scall ret a bl) F0)
+(* (HR : RA_normal R =
+     (fun rho0 : environ =>
+      EX  old : val,
+      substopt ret old F rho0 * maybe_retval (Q ts x) retty ret rho0))*)
+(HR: ( (ALL rho' : environ ,
+       !((EX old:val, substopt ret old F rho' * maybe_retval (Q ts x) retty ret rho') >=> (RA_normal R rho') ))) (m_phi jm))
+
+ (HGG:  genv_cenv psi = cenv_cs)
+ (H0 : rho = construct_rho (filter_genv psi) vx tx)
+ (H3 : eval_expr a rho = Vptr b Ptrofs.zero)
+ (H4 : (funassert Delta rho) (m_phi jm))
+ (H1 : (rguard Espec psi Delta
+        (frame_ret_assert R F0) k) (level (m_phi jm)))
+ (H11 : forall vl : environ, (!|>(Q' ts x vl <=> Q ts x vl)) (m_phi jm))
+ (H14 : (|>(F0 rho * F rho *
+          P ts x
+            (make_args (map fst params)
+               (eval_exprlist (map snd params) bl rho) rho))) (m_phi jm))
+ (n : nat)
+ (H2 : level (m_phi jm) = S n)
+ (H15 : (believe_external Espec psi (Vptr b Ptrofs.zero) (params, retty) cc A P Q')
+        (level (m_phi jm))),
+ exists (c' : corestate) (m' : juicy_mem),
+  jstep (cl_core_sem psi) (State vx tx (Kseq (Scall ret a bl) :: k)) jm c' m' /\
+  jm_bupd ora (jsafeN OK_spec psi n ora c') m'.
+Proof.
+intros. apply now_later in H1. apply now_later in HR.
+eapply semax_call_external; try eassumption; trivial.
 Qed.
 
 Lemma alloc_juicy_variables_age:
@@ -2329,14 +2505,19 @@ Lemma semax_call_aux:
     guard_environ Delta (current_function k) rho ->
     (snd fsig0 =Tvoid -> ret=None) ->
     closed_wrt_modvars (Scall ret a bl) F0 ->
-    RA_normal R = (fun rho0 : environ => EX old:val, substopt ret old F rho0 * maybe_retval (Q ts x) (snd fsig0) ret rho0) ->
+
+    (*LENB: replaced equality with entailment -- notice the |>
+       RA_normal R = (fun rho0 : environ => EX old:val, substopt ret old F rho0 * maybe_retval (Q ts x) (snd fsig0) ret rho0) ->*)
+    ( ( ALL rho' : environ , |>
+       !((EX old:val, substopt ret old F rho' * maybe_retval (Q ts x) (snd fsig0) ret rho') >=> (RA_normal R rho') )) (m_phi jm)) ->
+
 (*    Forall (fun it => complete_type (composite_types Delta) (snd it) = true) (fn_vars (snd fsig)) ->*)
     genv_cenv psi = cenv_cs ->
     rho = construct_rho (filter_genv psi) vx tx ->
     (*filter_genv psi = ge_of rho ->*)
     eval_expr a rho = Vptr b Ptrofs.zero ->
     (funassert Delta rho) (m_phi jm) ->
-    (rguard Espec psi Delta (frame_ret_assert R F0) k) (level (m_phi jm)) ->
+    (*LENB: now with a |> here*) (|> rguard Espec psi Delta (frame_ret_assert R F0) k) (level (m_phi jm)) ->
     (believe Espec Delta psi Delta) (level (m_phi jm)) ->
     (glob_specs Delta)!id = Some (mk_funspec fsig0 cc A P Q' NEP NEQ') ->
     Genv.find_symbol psi id = Some b ->
@@ -2377,8 +2558,8 @@ destruct fsig as [params retty].
 simpl @fst in *; simpl @snd in *.
 rewrite @snd_split in *.
 clear LATER.
-
-edestruct semax_call_external; eauto.
+(*apply now_later in H1.*)
+edestruct semax_call_external; eauto. { rewrite box_all. eassumption. } 
 destruct H5 as [? [? ?]].
 inv H5.
 econstructor; eauto.
@@ -2391,13 +2572,13 @@ destruct H15 as [b' [f [[? [? [COMPLETE [? ?]]]] ?]]].
 destruct H18 as [H17' [Hvars [H18 H18']]].
 inversion H15; clear H15; subst b'.
 
-assert (HDelta: forall f : function, tycontext_subsume (func_tycontext' f Delta) (func_tycontext' f Delta)).
-{ simpl; intros; apply tycontext_subsume_refl. }
+assert (HDelta: forall f : function, tycontext_sub (func_tycontext' f Delta) (func_tycontext' f Delta)).
+{ simpl; intros; apply tycontext_sub_refl. }
 specialize (H19 Delta (level (m_phi jm)) (necR_refl _) HDelta ts x n LATER).
 rewrite semax_fold_unfold in H19.
 apply (pred_nec_hereditary _ _ n (laterR_necR LATER)) in Prog_OK.
 pose (F0F := fun _: environ => F0 rho * F rho).
-specialize (H19 _ _ _ (necR_refl _) (conj (tycontext_subsume_refl _) HGG)  _ (necR_refl _) (Prog_OK)
+specialize (H19 _ _ _ (necR_refl _) (conj (tycontext_sub_refl _) HGG)  _ (necR_refl _) (Prog_OK)
                       ((*Kseq (Sreturn None) ::*) Kcall ret f (vx) (tx) :: k)
                        F0F _ (necR_refl _)).
 unfold F0F in *; clear F0F.
@@ -2470,16 +2651,59 @@ pose (rval := match vl with Some v => v | None => Vundef end).
 pose (te2 := match ret with
             | None => tx
             | Some rid => PTree.set rid rval tx
-            end).
+            end). (*
 specialize (H1 EK_normal None te2 vx).
 rewrite proj_frame_ret_assert in H1.
-simpl proj_ret_assert in H1.
-rewrite HR in H1; clear R HR. simpl exit_cont in H1.
-unfold seplog.sepcon,  seplog.LiftSepLog  in H1.
-specialize (H1 (m_phi jm2)).
+simpl proj_ret_assert in H1.*)
+
+assert (LATER2': (n >= level (m_phi jm2))%nat). { repeat rewrite <- level_juice_level_phi in *. omega. } 
+
+assert (HH1 : forall a' : rmap,
+     necR (m_phi jm2) a' ->
+     (!! guard_environ Delta (current_function k) (construct_rho (filter_genv psi) vx te2) &&
+      seplog.sepcon (fun rho0 : environ => EX old : val, substopt ret old F rho0 * maybe_retval (Q ts x) (snd fsig) ret rho0) F0
+        (construct_rho (filter_genv psi) vx te2) && funassert Delta (construct_rho (filter_genv psi) vx te2)) a' ->
+     (assert_safe Espec psi vx te2 (exit_cont EK_normal None k) (construct_rho (filter_genv psi) vx te2)) a').
+{ intros. clear Prog_OK. hnf in H1.
+  assert (Help0: laterM (level (m_phi jm)) (level (m_phi jm2))). { clear - LATER2' H2. rewrite <- ! level_juice_level_phi. rewrite H2; clear H2. simpl. apply later_nat. omega. }
+  specialize (H1 _ Help0 EK_normal None te2 vx); hnf in H1.
+  assert (Help1: (level (m_phi jm2) >= level (m_phi jm2))%nat) by omega. (* { clear - LATER2' H2. rewrite <- ! level_juice_level_phi in *.  omega. }*)
+  apply (H1 _ Help1 _ H21).
+  rewrite proj_frame_ret_assert in H1.
+  simpl proj_ret_assert in H1.
+  rewrite proj_frame_ret_assert.
+  simpl proj_ret_assert.
+  destruct H24 as [[XX1 XX2] XX3]. split; trivial. split; trivial. clear XX1 XX3.
+  destruct XX2 as [u1 [u2 [JU [U1 U2]]]]; destruct (join_level _ _ _ JU) as [LevU1 _].
+  exists u1, u2; split. trivial. split; [clear U2| trivial].
+  assert (JMX: laterM (m_phi jm) (m_phi jmx)). { constructor. apply age_jm_phi. apply H13. }
+  assert (JMX_u1: (level (m_phi jmx) >= level u1)%nat).
+  { rewrite LevU1; clear -H21 LATER2' H2 H13. apply necR_level in H21. apply age_level in H13.
+    rewrite H13 in H2. clear H13. inv H2. omega. }
+  apply (HR (construct_rho (filter_genv psi) vx te2) _ JMX _ JMX_u1 _ (necR_refl _) U1). }
+clear H1; rename HH1 into H1.
+(*assert (HH1 : forall a' : rmap,
+     necR (m_phi jm2) a' ->
+     (!! guard_environ Delta (current_function k) (construct_rho (filter_genv psi) vx te2) &&
+      seplog.sepcon (fun rho0 : environ => EX old : val, substopt ret old F rho0 * maybe_retval (Q ts x) (snd fsig) ret rho0) F0
+        (construct_rho (filter_genv psi) vx te2) && funassert Delta (construct_rho (filter_genv psi) vx te2)) a' ->
+     (assert_safe Espec psi vx te2 (exit_cont EK_normal None k) (construct_rho (filter_genv psi) vx te2)) a').
+{ intros. clear Prog_OK. hnf in H1.
+  assert (Help1: (level (m_phi jm) >= level (m_phi jm2))%nat). { clear - LATER2' H2. rewrite <- ! level_juice_level_phi in *.  omega. }
+  apply (H1 _ Help1 _ H21).
+  destruct H24 as [[XX1 XX2] XX3]. split; trivial. split; trivial. clear XX1 XX3.
+  destruct XX2 as [u1 [u2 [JU [U1 U2]]]]; destruct (join_level _ _ _ JU) as [LevU1 _].
+  exists u1, u2; split. trivial. split; [clear U2| trivial].
+  assert (JMX: laterM (m_phi jm) (m_phi jmx)). { constructor. apply age_jm_phi. apply H13. }
+  assert (JMX_u1: (level (m_phi jmx) >= level u1)%nat).
+  { rewrite LevU1; clear -H21 LATER2' H2 H13. apply necR_level in H21. apply age_level in H13.
+    rewrite H13 in H2. clear H13. inv H2. omega. }
+  apply (HR (construct_rho (filter_genv psi) vx te2) _ JMX _ JMX_u1 _ (necR_refl _) U1). }
+clear H1; rename HH1 into H1.*)
+(*
 spec H1.
 clear - FL3 H2 H23.
-repeat rewrite <- level_juice_level_phi in *. omega.
+repeat rewrite <- level_juice_level_phi in *. omega.*)
 specialize (H1 _ (necR_refl _)). simpl in H15.
 spec H1; [clear H1 | ].
 split; [split(*; [split |]*) |].
@@ -2502,11 +2726,11 @@ specialize (TC5 (eq_refl _)); congruence.
 rewrite <- H0. auto.
 }
 {
- destruct H22 as [H22a H22b].
- rewrite seplog.sepcon_comm.
- rewrite <- exp_sepcon1.
+ destruct H22 as [H22a H22b].  (*rewrite ! sepcon_assoc in H22a.
+ rewrite seplog.sepcon_comm. destruct H22a as [u1 [u2 [JU [U1 U2]]]]; destruct (join_level _ _ _ JU) as [Levu1 Levu2].*)
+ (*rewrite <- exp_sepcon1.*)
  simpl seplog.sepcon.
-  rewrite <- sepcon_assoc.
+(*  rewrite <- sepcon_assoc.*)
  rewrite sepcon_comm in H22a|-*.
   rewrite sepcon_assoc in H22a.
  assert (bind_ret vl (fn_return f) (Q ts x) rho' * (F0 rho * F rho)
@@ -2517,7 +2741,7 @@ apply sepcon_derives.
 *
  clear dependent a. clear H11 H19 H20 H10 H9 H12 H5 H6 H8.
  clear Prog_OK ora ora'.  subst rho' fsig.
- clear H22b VR. clear FL jm2 FL2 FL3.
+ clear H22b VR. clear LATER2' FL jm2 FL2 FL3.
  clear b H16 H7. clear bl TC2 H14.
  unfold te2; clear te2. unfold rval; clear rval.
  unfold bind_ret.
@@ -2566,9 +2790,11 @@ apply sepcon_derives.
   apply H0. rewrite PTree.gso; auto.
 +
   apply exp_right with Vundef; simpl; auto.
-}
- apply H1; clear H1.
- eapply free_list_juicy_mem_lem; eauto.
+} 
+  eapply derives_trans. 3: apply H1. apply derives_refl.
+  normalize. intros v. exists v. rewrite <- sepcon_assoc. rewrite sepcon_comm in H21. apply H21.
+  (*apply H1; clear H1.*)
+ eapply free_list_juicy_mem_lem. eauto.
  eapply sepcon_derives; try apply H22a; auto.
 }
 {
@@ -2834,14 +3060,53 @@ apply age_level in H20x.
 rewrite <- level_juice_level_phi in *; congruence.
 Qed.
 
-Lemma func_at_func_at':
- forall fs loc, func_at fs loc |-- func_at' fs loc.
-Proof.
-unfold func_at, func_at'; destruct fs; intros. hnf; intros.
-eexists; eauto.
-Qed.
 
-Lemma semax_call:
+Lemma semax_call_aux':
+ forall (Delta : tycontext)
+  (A : TypeTree)
+  (P Q Q' : forall ts, dependent_type_functor_rec ts (AssertTT A) mpred)
+  (NEP: super_non_expansive P) (NEQ': super_non_expansive Q')
+  (ts: list Type) (x : dependent_type_functor_rec ts A mpred)
+  (F : environ -> pred rmap)
+  (F0 : assert) (ret : option ident) (fsig0 : funsig) cc (a : expr)
+  (bl : list expr) (R : ret_assert) (psi : genv) (vx:env) (tx:Clight.temp_env) (k : cont) (rho : environ)
+  (ora : OK_ty) (jm : juicy_mem) (b : block) (id : ident),
+   Cop.classify_fun (typeof a) =
+   Cop.fun_case_f (type_of_params (fst fsig0)) (snd fsig0) cc ->
+   tc_fn_return Delta ret (snd fsig0) ->
+   (|>tc_expr Delta a rho) (m_phi jm) ->
+   (|>tc_exprlist Delta (snd (split (fst fsig0))) bl rho) (m_phi jm) ->
+    (*map typeof bl = map (@snd _ _) (fst fsig) ->*)
+    guard_environ Delta (current_function k) rho ->
+    (snd fsig0 =Tvoid -> ret=None) ->
+    closed_wrt_modvars (Scall ret a bl) F0 ->
+
+    (*RA_normal R = (fun rho0 : environ => EX old:val, substopt ret old F rho0 * maybe_retval (Q ts x) (snd fsig0) ret rho0) ->*)
+    ( (ALL rho' : environ ,
+       !((EX old:val, substopt ret old F rho' * maybe_retval (Q ts x) (snd fsig0) ret rho') >=> (RA_normal R rho') )) (m_phi jm)) ->
+
+(*    Forall (fun it => complete_type (composite_types Delta) (snd it) = true) (fn_vars (snd fsig)) ->*)
+    genv_cenv psi = cenv_cs ->
+    rho = construct_rho (filter_genv psi) vx tx ->
+    (*filter_genv psi = ge_of rho ->*)
+    eval_expr a rho = Vptr b Ptrofs.zero ->
+    (funassert Delta rho) (m_phi jm) ->
+    (rguard Espec psi Delta (frame_ret_assert R F0) k) (level (m_phi jm)) ->
+    (believe Espec Delta psi Delta) (level (m_phi jm)) ->
+    (glob_specs Delta)!id = Some (mk_funspec fsig0 cc A P Q' NEP NEQ') ->
+    Genv.find_symbol psi id = Some b ->
+    (forall vl : environ, (!|>(Q' ts x vl <=> Q ts x vl)) (m_phi jm)) ->
+    (|>(F0 rho * F rho *
+           P ts x (make_args (map (@fst  _ _) (fst fsig0))
+             (eval_exprlist (snd (split (fst fsig0))) bl rho) rho)
+            )) (m_phi jm) ->
+   jsafeN (@OK_spec Espec) psi (level (m_phi jm)) ora
+     (State (vx) (tx) (Kseq (Scall ret a bl) :: k)) jm.
+Proof. intros. apply now_later in H6. apply now_later in H11. rewrite box_all in H6.
+eapply semax_call_aux; try eassumption; try trivial.
+Qed. 
+
+Lemma semax_call_weak:
   forall Delta (A: TypeTree)
   (P Q : forall ts, dependent_type_functor_rec ts (AssertTT A) mpred)
   (NEP: super_non_expansive P) (NEQ: super_non_expansive Q)
@@ -2853,7 +3118,7 @@ Lemma semax_call:
           tc_fn_return Delta ret retsig ->
   semax Espec Delta
        (fun rho => (|>(tc_expr Delta a rho && tc_exprlist Delta (snd (split argsig)) bl rho))  &&
-           (func_ptr (mk_funspec (argsig,retsig) cc A P Q NEP NEQ) (eval_expr a rho) &&
+           (func_ptr_weak (mk_funspec (argsig,retsig) cc A P Q NEP NEQ) (eval_expr a rho) &&
           (|>(F rho * P ts x (make_args (map (@fst  _ _) argsig)
                 (eval_exprlist (snd (split argsig)) bl rho) rho )))))
          (Scall ret a bl)
@@ -2885,11 +3150,12 @@ assert (TC7': tc_fn_return Delta' ret retsig).
   destruct H; auto.
   auto.
 } clear TC7.
-
 rewrite !later_andp in H0.
 apply extend_sepcon_andp in H0; auto.
 destruct H0 as [[TC1 TC2] pre].
-normalize in pre. unfold func_ptr in *.
+
+normalize in pre. unfold func_ptr_weak in *. hnf in pre.
+destruct pre as [z1 [z2 [JZ [HF0 pre]]]].
 destruct pre as [[b [EvalA funcatb]] HP].
 destruct (level w) eqn: Hl.
 { apply own.bupd_intro; repeat intro.
@@ -2898,47 +3164,55 @@ rewrite <- Hl in *.
 destruct (levelS_age w n) as (w' & Hage & Hw'); auto.
 
 hnf in funcatb. 
-(*Here
-specialize (funassertDelta (b) (mk_funspec (argsig,retsig) cc A P Q NEP NEQ) _ (necR_refl _)).
-spec H7.
-1: apply func_at_func_at'; apply H6.*)
-assert (XX: exists id:ident, (Map.get (ge_of (construct_rho (filter_genv psi) vx tx)) id = Some b)
-                             /\ exists fs, (glob_specs Delta')!id = Some fs).
-{ destruct funassertDelta' as [_ FD]. apply (FD b (argsig, retsig) cc _ (necR_refl _)).
-  simpl. eexists; eapply funcatb. }
-destruct XX as [id [Hb [fs specID]]]; simpl in Hb.
-destruct funassertDelta' as [funassertDeltaA funassertDeltaB].
 
-destruct (funassertDeltaA id fs _ (necR_refl _) specID) as [v [Hv funcatv]]; simpl in Hv.
-assert (VB: b=v); [inversion2 Hb Hv; trivial | subst; clear Hb].
-unfold func_at in funcatv.
-destruct fs as [fsig' cc' A' P' Q' NEP' NEQ'].
-hnf in funcatb, funcatv.
-inversion2 funcatv funcatb; clear funcatv.
-apply inj_pair2 in H3; rename H3 into HSpecs.
-destruct (function_pointer_aux A' P P' Q Q' w NEP NEQ NEP' NEQ') as [Hpre Hpost]; [f_equal; apply HSpecs | clear HSpecs].
+destruct funcatb as [gs [GS funcatb]]. simpl in GS.
+assert (funcatb_w: (func_at gs (b, 0)) w). 
+{ clear - JZ funcatb. specialize (corable_func_at gs (b,0)); intros. 
+  forget (func_at gs (b,0)) as P. rewrite corable_spec in H. 
+  apply (H z2); trivial. apply join_comm in JZ. eapply join_core. apply JZ. }
+unfold func_at, pureat in funcatb_w.
 
 assert (Hpsi: filter_genv psi = ge_of (construct_rho (filter_genv psi) vx tx)) by reflexivity.
 unfold filter_genv in Hpsi.
 remember (construct_rho (filter_genv psi) vx tx) as rho.
 set (args := eval_exprlist (snd (split argsig)) bl rho).
-fold args in HP. clear Hpsi.
 
-specialize (Hpre ts x (make_args (map (@fst  _ _) argsig) (eval_exprlist (snd (split argsig))bl rho) rho)).
-specialize (Hpost ts x).
-assert (ArgsW: app_pred (|> (F0 rho * F rho * P' ts x (make_args (map (@fst  _ _) argsig)
-  (eval_exprlist (snd (split argsig)) bl rho) rho))) w).
-{
-  do 3 red in Hpre.
-  apply eqp_later1 in Hpre.
-  apply pred_eq_e2 in Hpre.
-  rewrite later_sepcon.
-  eapply (sepcon_subp' (|>(F0 rho * F rho)) _ (|> P ts x (make_args (map (@fst  _ _) argsig) (eval_exprlist (snd (split argsig)) bl rho) rho)) _ (level w)); eauto.
-  rewrite <- later_sepcon, sepcon_assoc, later_sepcon.
-  eapply derives_e, HP.
-  apply sepcon_derives, derives_refl; apply now_later.
-}
-clear Hpre.
+(*Here
+specialize (funassertDelta (b) (mk_funspec (argsig,retsig) cc A P Q NEP NEQ) _ (necR_refl _)).
+spec H7.
+1: apply func_at_func_at'; apply H6.*)
+
+assert (MYPROP: exists id fs, Map.get (ge_of rho) id = Some b /\ 
+         (glob_specs Delta') ! id = Some fs /\ func_at fs (b, 0) w).
+{ clear - funcatb_w funassertDelta' GS JZ.
+  assert (XX: exists id:ident, (Map.get (ge_of rho) id = Some b)
+                               /\ exists fs, (glob_specs Delta')!id = Some fs).
+  { destruct funassertDelta' as [_ FD]. 
+    apply (FD b (argsig, retsig) cc _ (necR_refl _)); clear FD.
+    simpl. destruct gs. hnf in funcatb_w. (*destruct GS as [[? ?] _]; subst.*) destruct GS as [? [? ?]]; subst.
+    eexists; eauto. }
+  destruct XX as [id [Hb [fs specID]]]; simpl in Hb.
+
+  assert (exists v, Map.get (ge_of rho) id = Some v /\ func_at fs (v, 0) w).
+  { destruct funassertDelta' as [funassertDeltaA _].
+    destruct (funassertDeltaA id fs _ (necR_refl _) specID) as [v [Hv funcatv]]; simpl in Hv.
+    exists v; split; trivial. }
+  destruct H as [v [Hv funcatv]].
+  assert (VB: b=v); [inversion2 Hb Hv; trivial | subst; clear Hb].
+  exists id, fs; auto. }
+destruct MYPROP as [id [fs [RhoID [SpecOfID funcatv]]]].
+destruct fs as [fsig' cc' A' P' Q' NEP' NEQ'].
+unfold func_at in funcatv, funcatb_w. destruct gs.
+hnf in funcatb_w, funcatv. inversion2 funcatv funcatb_w.
+assert (PREPOST: (forall ts x vl, (! |> (P' ts x vl <=> P0 ts x vl)) w) /\
+                 (forall ts x vl, (! |> (Q' ts x vl <=> Q0 ts x vl)) w)).
+{ apply inj_pair2 in H3; 
+  apply (function_pointer_aux); trivial. f_equal; apply H3. }
+clear H3; destruct PREPOST as [Hpre Hpost]. 
+
+fold args in HP. clear Hpsi. remember (construct_rho (filter_genv psi) vx tx) as rho; clear Heqrho.
+(*destruct GS as [[? ?] GS]*) destruct GS as [? [? GS]]; subst fsig' cc'.
+
 assert (typecheck_environ Delta rho) as TC4.
 { clear - TC3 TS.
   destruct TC3 as [TC3 TC4].
@@ -2948,12 +3222,536 @@ assert (typecheck_environ Delta rho) as TC4.
 eapply later_derives in TC2; [|apply (tc_exprlist_sub _ _ _ TS); auto].
 eapply later_derives in TC1; [|apply (tc_expr_sub _ _ _ TS); auto].
 clear TC4.
+
+assert (HPP: (|> (F0 rho * F rho * P ts x (make_args (map fst argsig) args rho)))%pred w).
+{ clear - HP JZ HF0. rewrite sepcon_assoc. rewrite later_sepcon. exists z1, z2; split; trivial. 
+  split. apply now_later; trivial. trivial. }
+simpl in EvalA.  clear funcatb HP JZ HF0 z1 z2.
+rewrite later_sepcon in HPP.
+destruct HPP as [w1 [w2 [J [W1 W2]]]]; destruct (join_level _ _ _ J) as [LevW1 LevW2].
+destruct (age1_join2 _ J Hage) as [w1' [w2' [J' [Age1 Age2]]]].
+
+assert (TRIV: (forall rho, typecheck_temp_environ rho (PTree.empty type)) /\
+              (typecheck_var_environ (Map.empty (block * type)) (PTree.empty type)) /\ 
+              (forall rho, typecheck_glob_environ rho (PTree.empty type))).
+{ clear. split.
+  { intros; hnf; intros. rewrite PTree.gempty in H; congruence. } split. 
+  { intros; hnf; intros. split; intros. rewrite PTree.gempty in H; congruence. 
+    destruct H. unfold Map.empty, Map.get in H; congruence. } 
+  { intros; hnf; intros. rewrite PTree.gempty in H; congruence. } }
+
+assert (TCD': tc_environ Delta' rho) by eapply TC3.
+
+assert (LA2: laterM w2 w2'). { constructor; trivial. }
+assert (TCARGS: tc_environ (funsig_tycontext (argsig, retsig)) (make_args (map fst argsig) args rho)).
+{ assert (LaterW': laterR w w'). constructor; trivial.
+  specialize (TC2 _ LaterW'). subst args.
+  apply (tc_environ_make_args' argsig retsig bl rho Delta' TCD' _ TC2).  }
  
+specialize (GS ts x (make_args (map fst argsig) args rho)).
+destruct (GS w2') as [ts1 [x1 [G [HG1 HG2]]]].
+{ simpl; split; trivial. clear - W2 Age2. apply W2. apply age_laterR; trivial. }
+
+specialize (Hpre ts1 x1 (make_args (map fst argsig) args rho)).
+
+assert (ArgsW: app_pred (|> (F0 rho * (F rho * G) * P' ts1 x1 (make_args (map (@fst  _ _) argsig)
+  (eval_exprlist (snd (split argsig)) bl rho) rho) )) w).
+{ clear Hpost HG2 funcatv SpecOfID Prog_OK RhoID TC7' RGUARD.
+  assert (XX: (|> (F0 rho * F rho * G * P' ts1 x1 (make_args (map (@fst  _ _) argsig)
+     (eval_exprlist (snd (split argsig)) bl rho) rho) )) w). 
+  { rewrite sepcon_assoc. rewrite sepcon_assoc. rewrite <- sepcon_assoc.
+    rewrite later_sepcon.
+    exists w1, w2; split. trivial. split. trivial. hnf; intros.
+    destruct (age_later Age2 H); [ subst a' |].
+    - destruct HG1 as [u1 [u2 [JU [U1 U2]]]]; destruct (join_level _ _ _ JU) as [LevU1 LevU2]. 
+      exists u1, u2; split; trivial. split; trivial. 
+      assert (LatWU2: laterM (level w) (level u2)). { rewrite LevU2, <- LevW2 . apply laterR_level'; trivial. }
+      eapply (Hpre (level u2) LatWU2); [| apply necR_refl | trivial]; omega.
+    - apply now_later in HG1. specialize (HG1 _ H0).
+      destruct HG1 as [u1 [u2 [JU [U1 U2]]]]; destruct (join_level _ _ _ JU) as [LevU1 LevU2]. 
+      exists u1, u2; split; trivial. split; trivial. 
+      assert (LatWU2: laterM (level w) (level u2)). { rewrite LevU2, <- LevW2 . apply laterR_level'; trivial. }
+      eapply (Hpre (level u2) LatWU2); [| apply necR_refl | trivial]; omega.  }
+  clear - XX. rewrite 2 sepcon_assoc. rewrite 2 sepcon_assoc in XX.
+  intros u U. destruct (XX _ U) as [u1 [u2 [J [U1 U2]]]]; clear XX.
+  exists u1, u2; split; trivial. split; trivial.
+}
+
+clear Hpre.
+specialize (Hpost ts1 x1).
 apply own.bupd_intro; repeat intro; subst.
-eapply semax_call_aux; try eassumption;
- try solve [simpl; eassumption].
-simpl RA_normal; auto.
-split; trivial.
+eapply semax_call_aux' with (F := fun rho => F rho * G)(P:=P')(F0:=F0)(rho:=construct_rho (filter_genv psi) vx tx)
+ (ts:=ts1)(x:=x1)(fsig0:=(argsig, retsig))(R:=(normal_ret_assert
+          (fun rho => (EX old:val, substopt ret old F rho * maybe_retval (Q ts x) retsig ret rho)))); try eassumption; try trivial.
+(*apply now_later.*)
+simpl RA_normal; auto. clear - TRIV TC7' HG2. change (snd (argsig, retsig)) with retsig.
+intros rho' u U m NEC [v V]. exists v.
+hnf in TC7'.
+destruct ret. 
++ remember ((temp_types Delta') ! i) as rr; destruct rr; try contradiction; subst t.
+  assert (TCR: tc_environ (ret0_tycon (funsig_tycontext (argsig, retsig))) (get_result1 i rho')).
+  { hnf; simpl. intuition. }
+  simpl in V; simpl. destruct V as [m1 [m2 [JM [[u1 [u2 [JU [U1 U2]]]] M2]]]].
+  destruct (join_assoc JU JM) as [q1 [Q2 Q1]].
+  exists u1, q1; split; trivial. split. apply U1.
+  hnf in HG2. apply HG2. simpl. split. trivial.
+  exists u2, m2; auto.
++ destruct V as [m1 [m2 [JM [[u1 [u2 [JU [U1 U2]]]] M2]]]].
+  destruct (join_assoc JU JM) as [q1 [Q2 Q1]]. simpl in M2. simpl.
+  exists u1, q1; split; trivial. split. apply U1.
+  hnf in HG2.
+  destruct retsig. 
+  - apply HG2. simpl. split. hnf; simpl; intuition. exists u2, m2; auto.
+  - destruct M2 as [z M2]; exists z. apply HG2. simpl. split; [ hnf; simpl; intuition | exists u2, m2; auto].
+  - destruct M2 as [z M2]; exists z. apply HG2. simpl. split; [ hnf; simpl; intuition | exists u2, m2; auto].
+  - destruct M2 as [z M2]; exists z. apply HG2. simpl. split; [ hnf; simpl; intuition | exists u2, m2; auto].
+  - destruct M2 as [z M2]; exists z. apply HG2. simpl. split; [ hnf; simpl; intuition | exists u2, m2; auto].
+  - destruct M2 as [zz M2]; exists zz. apply HG2. simpl. split; [ hnf; simpl; intuition | exists u2, m2; auto].
+  - destruct M2 as [z M2]; exists z. apply HG2. simpl. split; [ hnf; simpl; intuition | exists u2, m2; auto].
+  - destruct M2 as [z M2]; exists z. apply HG2. simpl. split; [ hnf; simpl; intuition | exists u2, m2; auto].
+  - destruct M2 as [z M2]; exists z. apply HG2. simpl. split; [ hnf; simpl; intuition | exists u2, m2; auto].
+Qed.
+
+Lemma semax_call:
+  forall Delta (A: TypeTree)
+  (P Q : forall ts, dependent_type_functor_rec ts (AssertTT A) mpred)
+  (NEP: super_non_expansive P) (NEQ: super_non_expansive Q)
+  (ts: list Type) (x : dependent_type_functor_rec ts A mpred)
+   F ret argsig retsig cc a bl,
+           Cop.classify_fun (typeof a) =
+           Cop.fun_case_f (type_of_params argsig) retsig cc ->
+            (retsig = Tvoid -> ret = None) ->
+          tc_fn_return Delta ret retsig ->
+  semax Espec Delta
+       (fun rho => (|>(tc_expr Delta a rho && tc_exprlist Delta (snd (split argsig)) bl rho))  &&
+           (func_ptr (mk_funspec (argsig,retsig) cc A P Q NEP NEQ) (eval_expr a rho) &&
+          (|>(F rho * P ts x (make_args (map (@fst  _ _) argsig)
+                (eval_exprlist (snd (split argsig)) bl rho) rho )))))
+         (Scall ret a bl)
+         (normal_ret_assert
+          (fun rho => (EX old:val, substopt ret old F rho * maybe_retval (Q ts x) retsig ret rho))).
+Proof.
+rewrite semax_unfold. intros ? ? ? ? ? ? ? ? ? ? ? ? ? ? ? TCF TC5 TC7.
+intros.
+rename H into Cloased; rename H0 into RGUARD. Locate guard.
+intros tx vx.
+intros ? ? ? NecR_ya' [[TC3 ?] funassertDelta'].
+
+assert (NecR_wa': necR w (level a')).
+{ apply nec_nat. apply necR_level in NecR_ya'. apply le_trans with (level y); auto. }
+eapply pred_nec_hereditary in RGUARD; [ | apply NecR_wa'].
+eapply pred_nec_hereditary in Prog_OK; [ | apply NecR_wa'].
+clear w NecR_wa' NecR_ya' y H.
+rename a' into w.
+
+
+assert (TC7': tc_fn_return Delta' ret retsig).
+{
+  clear - TC7 TS.
+  hnf in TC7|-*. destruct ret; auto.
+  destruct ((temp_types Delta) ! i) eqn:?; try contradiction.
+  destruct TS.
+  specialize (H i); rewrite Heqo in H. subst t.
+  destruct ((temp_types Delta') ! i ).
+  destruct H; auto.
+  auto.
+} (*clear TC7.*)
+rewrite !later_andp in H0.
+apply extend_sepcon_andp in H0; auto.
+destruct H0 as [[TC1 TC2] pre].
+
+normalize in pre. unfold func_ptr in *.
+destruct pre as [[b [EvalA funcatb]] HP].
+destruct (level w) eqn: Hl.
+{ apply own.bupd_intro; repeat intro.
+  rewrite Hl; constructor. }
+rewrite <- Hl in *.
+destruct (levelS_age w n) as (w' & Hage & Hw'); auto.
+
+hnf in funcatb. 
+
+destruct funcatb as [gs [GS funcatb]].
+
+assert (Hpsi: filter_genv psi = ge_of (construct_rho (filter_genv psi) vx tx)) by reflexivity.
+unfold filter_genv in Hpsi.
+remember (construct_rho (filter_genv psi) vx tx) as rho.
+set (args := eval_exprlist (snd (split argsig)) bl rho).
+
+(*Here
+specialize (funassertDelta (b) (mk_funspec (argsig,retsig) cc A P Q NEP NEQ) _ (necR_refl _)).
+spec H7.
+1: apply func_at_func_at'; apply H6.*)
+
+assert (MYPROP: exists id fs, Map.get (ge_of rho) id = Some b /\ 
+         (glob_specs Delta') ! id = Some fs /\ func_at fs (b, 0) w).
+{ clear - funcatb funassertDelta' GS.
+  assert (XX: exists id:ident, (Map.get (ge_of rho) id = Some b)
+                               /\ exists fs, (glob_specs Delta')!id = Some fs).
+  { destruct funassertDelta' as [_ FD]. 
+    apply (FD b (argsig, retsig) cc _ (necR_refl _)); clear FD.
+    simpl. destruct gs. hnf in funcatb. destruct GS as [[? ?] _]; subst. (* destruct GS as [? [? ?]]; subst.*)
+    eexists. eapply funcatb. }
+  destruct XX as [id [Hb [fs specID]]]; simpl in Hb.
+
+  assert (exists v, Map.get (ge_of rho) id = Some v /\ func_at fs (v, 0) w).
+  { destruct funassertDelta' as [funassertDeltaA _].
+    destruct (funassertDeltaA id fs _ (necR_refl _) specID) as [v [Hv funcatv]]; simpl in Hv.
+    exists v; split; trivial. }
+  destruct H as [v [Hv funcatv]].
+  assert (VB: b=v); [inversion2 Hb Hv; trivial | subst; clear Hb].
+  exists id, fs; auto. }
+destruct MYPROP as [id [fs [RhoID [SpecOfID funcatv]]]].
+destruct fs as [fsig' cc' A' P' Q' NEP' NEQ'].
+unfold func_at in funcatv, funcatb. destruct gs.
+hnf in funcatb, funcatv. inversion2 funcatv funcatb.
+assert (PREPOST: (forall ts x vl, (! |> (P' ts x vl <=> P0 ts x vl)) w) /\
+                 (forall ts x vl, (! |> (Q' ts x vl <=> Q0 ts x vl)) w)).
+{ apply inj_pair2 in H3; 
+  apply (function_pointer_aux); trivial. f_equal; apply H3. }
+clear H3; destruct PREPOST as [Hpre Hpost]. 
+
+fold args in HP. clear Hpsi. remember (construct_rho (filter_genv psi) vx tx) as rho.
+
+assert (typecheck_environ Delta rho) as TC4.
+{ clear - TC3 TS.
+  destruct TC3 as [TC3 TC4].
+  eapply typecheck_environ_sub in TC3; [| eauto].
+  auto.
+} 
+eapply later_derives in TC2; [|apply (tc_exprlist_sub _ _ _ TS); auto].
+eapply later_derives in TC1; [|apply (tc_expr_sub _ _ _ TS); auto].
+clear TC4.
+
+assert (TCD': tc_environ Delta' rho) by eapply TC3.
+
+assert (TCARGS: tc_environ (funsig_tycontext (argsig, retsig)) (make_args (map fst argsig) args rho)).
+{ assert (LaterW': laterR w w'). constructor; trivial.
+  specialize (TC2 _ LaterW'). subst args.
+  apply (tc_environ_make_args' argsig retsig bl rho Delta' TCD' _ TC2).  }
+
+clear Heqrho.
+destruct GS as [[? ?] GS] (* destruct GS as [? [? GS]]*); subst fsig' cc'.
+
+rewrite later_sepcon, <- sepcon_assoc in HP.
+
+assert (HPP: (|> (F0 rho * F rho * P ts x (make_args (map fst argsig) args rho)))%pred w).
+{ clear - HP. rewrite 2 later_sepcon. rewrite sepcon_assoc.  rewrite sepcon_assoc in HP. 
+  eapply sepcon_derives. 3: apply HP. apply now_later. trivial. } clear HP.
+rewrite later_sepcon in HPP.
+destruct HPP as [w1 [w2 [J [W1 W2]]]]; destruct (join_level _ _ _ J) as [LevW1 LevW2].
+destruct (age1_join2 _ J Hage) as [w1' [w2' [J' [Age1 Age2]]]]; destruct (join_level _ _ _ J') as [Lw1' Lw2'].
+
+assert (LA2: laterM w2 w2'). { constructor; trivial. }
+(*specialize (Hpre ts).*)
+specialize (GS ts). hnf in GS.
+fold (@dependent_type_functor_rec ts) in *.
+specialize (W2 _ LA2). 
+
+specialize (GS x (make_args (map fst argsig) args rho)). hnf in GS.
+assert (LW2': (level w >= level w2')%nat). { apply age_level in Age2. destruct (join_level _ _ _ J); omega. }
+destruct (GS _ LW2' _ (necR_refl _)) as [ts1 [x1 [G [AA BB]]]]; clear GS.
+{ split; trivial. } 
+
+specialize (Hpre ts1 x1 (make_args (map fst argsig) args rho)).
+fold (@dependent_type_functor_rec ts1) in *.
+rewrite <- later_unfash in Hpre.
+specialize (Hpre _ (age_laterR Hage)).
+(****)
+
+
+destruct AA as [u1 [u2 [JU [U1 U2]]]]; destruct (join_level _ _ _ JU) as [Lu1 Lu2].
+hnf in Hpre. destruct (Hpre u2) as [_ HP']; clear Hpre. omega. specialize (HP' _ (necR_refl _) U2).
+
+assert (ArgsW: app_pred (|> (F0 rho * (F rho * G) * P' ts1 x1 (make_args (map (@fst  _ _) argsig)
+  (eval_exprlist (snd (split argsig)) bl rho) rho) )) w).
+{ clear Hpost funcatv SpecOfID Prog_OK RhoID TC7' RGUARD.
+  assert (XX: (|> (F0 rho * F rho * G * P' ts1 x1 (make_args (map (@fst  _ _) argsig)
+     (eval_exprlist (snd (split argsig)) bl rho) rho) )) w). 
+  { rewrite sepcon_assoc. rewrite sepcon_assoc. rewrite <- sepcon_assoc.
+    rewrite later_sepcon.
+    exists w1, w2; split. trivial. split. trivial. hnf; intros. specialize (age_later_nec _ _ _ Age2 H). intros.
+    destruct (nec_join2  JU H0) as [a1' [a2' [JA [A1 A2]]]]; destruct (join_level _ _ _ JA) as [La1 La2].
+    exists a1', a2'; split. trivial. split.
+    + destruct (nec_refl_or_later _ _ A1); subst. trivial. eapply now_later. apply U1. trivial. 
+    + destruct (nec_refl_or_later _ _ A2); subst. trivial. eapply now_later. apply HP'. trivial. }
+  clear - XX. rewrite 2 sepcon_assoc. rewrite 2 sepcon_assoc in XX.
+  intros u U. destruct (XX _ U) as [u1 [u2 [J [U1 U2]]]]; clear XX.
+  exists u1, u2; split; trivial. split; trivial. 
+}
+apply now_later in  RGUARD.
+apply own.bupd_intro; repeat intro; subst.
+eapply semax_call_aux with (F := fun rho => F rho * G)(P:=P')(F0:=F0)(rho:=construct_rho (filter_genv psi) vx tx)
+ (ts:=ts1)(x:=x1)(fsig0:=(argsig, retsig));  try eassumption; try trivial.
+
+simpl RA_normal; auto. clear ArgsW Hpost RGUARD ora. 
+(*assert ((ALL rho' : environ , |>
+ ! ((EX old : val,
+     substopt ret old (fun rho : environ => F rho * G) rho' * maybe_retval (Q0 ts1 x1) (snd (argsig, retsig)) ret rho') >=>
+    (EX old : val, substopt ret old F rho' * maybe_retval (Q ts x) retsig ret rho'))) (m_phi jm)).
+{*) intros rho' l L y Y z YZ [v Z]. exists v.
+assert (TRIV: (forall rho, typecheck_temp_environ rho (PTree.empty type)) /\
+              (typecheck_var_environ (Map.empty (block * type)) (PTree.empty type)) /\ 
+              (forall rho, typecheck_glob_environ rho (PTree.empty type))).
+{ clear. split.
+  { intros; hnf; intros. rewrite PTree.gempty in H; congruence. } split. 
+  { intros; hnf; intros. split; intros. rewrite PTree.gempty in H; congruence. 
+    destruct H. unfold Map.empty, Map.get in H; congruence. } 
+  { intros; hnf; intros. rewrite PTree.gempty in H; congruence. } }
+assert (LEV2': (level w2' >= level w2')%nat) by omega. 
+assert (LEVz: (level w2' >= level z)%nat). 
+{ rewrite Lw2'. apply necR_level in YZ.
+  destruct (age_later Hage L).
+  + subst l; omega. + apply laterR_level in H; omega. }
+destruct ret; simpl.
++ destruct Z as [z1 [z2 [JZ [Z1 Z2]]]]; destruct (join_level _ _ _ JZ) as [Levz1 Levz2]. simpl in Z1, Z2.
+  destruct Z1 as [z1_1 [z1_2 [JZ1 [Z11 Z12]]]]; destruct (join_level _ _ _ JZ1) as [Levz11 Levz12].
+  destruct (join_assoc JZ1 JZ) as [y11 [JY1 JY2]]; destruct (join_level _ _ _ JY2) as [_ Levy11].
+  assert (LL: (level w2' >= level y11)%nat) by omega. 
+  exists z1_1, y11; split; trivial. split; trivial.
+  apply (BB (get_result1 i rho') _ LL _ (necR_refl _)).
+  simpl; split. { hnf; simpl; intuition. }
+  exists z1_2, z2; auto.
++ destruct Z as [z1 [z2 [JZ [Z1 Z2]]]]; destruct (join_level _ _ _ JZ) as [Levz1 Levz2]. simpl in Z1, Z2.
+  destruct Z1 as [z1_1 [z1_2 [JZ1 [Z11 Z12]]]]; destruct (join_level _ _ _ JZ1) as [Levz11 Levz12].
+  destruct (join_assoc JZ1 JZ) as [y11 [JY1 JY2]]; destruct (join_level _ _ _ JY2) as [_ Levy11].
+  assert (LL: (level w2' >= level y11)%nat) by omega. 
+  exists z1_1, y11; split; trivial. split; trivial. 
+  destruct (type_eq retsig Tvoid).
+  - subst retsig. 
+    apply (BB (globals_only rho') _ LL _ (necR_refl _)).
+    simpl; split. hnf; simpl; intuition.
+    exists z1_2, z2; auto.
+  - assert (Z22: ((fun rho : environ => EX v : val, Q0 ts1 x1 (env_set (globals_only rho) ret_temp v)) rho') z2).
+    destruct retsig; trivial.  congruence.
+    clear Z2; destruct Z22 as [vv Z2]. 
+    specialize (BB (env_set (globals_only rho') ret_temp vv) _ LL _ (necR_refl _)); spec BB.
+    * simpl; split. hnf; simpl; intuition.
+      exists z1_2, z2; auto.
+    *  destruct retsig; try solve [ congruence]; exists vv; trivial.
+Qed.
+
+Lemma semax_call_early:
+  forall Delta (A: TypeTree)
+  (P Q : forall ts, dependent_type_functor_rec ts (AssertTT A) mpred)
+  (NEP: super_non_expansive P) (NEQ: super_non_expansive Q)
+  (ts: list Type) (x : dependent_type_functor_rec ts A mpred)
+   F ret argsig retsig cc a bl,
+           Cop.classify_fun (typeof a) =
+           Cop.fun_case_f (type_of_params argsig) retsig cc ->
+            (retsig = Tvoid -> ret = None) ->
+          tc_fn_return Delta ret retsig ->
+  semax Espec Delta
+       (fun rho => (|>(tc_expr Delta a rho && tc_exprlist Delta (snd (split argsig)) bl rho))  &&
+           (func_ptr_early (mk_funspec (argsig,retsig) cc A P Q NEP NEQ) (eval_expr a rho) &&
+          (|>(F rho * P ts x (make_args (map (@fst  _ _) argsig)
+                (eval_exprlist (snd (split argsig)) bl rho) rho )))))
+         (Scall ret a bl)
+         (normal_ret_assert
+          (fun rho => (EX old:val, substopt ret old F rho * maybe_retval (Q ts x) retsig ret rho))).
+Proof.
+rewrite semax_unfold. intros ? ? ? ? ? ? ? ? ? ? ? ? ? ? ? TCF TC5 TC7.
+intros.
+rename H into Cloased; rename H0 into RGUARD. Locate guard.
+intros tx vx.
+intros ? ? ? NecR_ya' [[TC3 ?] funassertDelta'].
+
+assert (NecR_wa': necR w (level a')).
+{ apply nec_nat. apply necR_level in NecR_ya'. apply le_trans with (level y); auto. }
+eapply pred_nec_hereditary in RGUARD; [ | apply NecR_wa'].
+eapply pred_nec_hereditary in Prog_OK; [ | apply NecR_wa'].
+clear w NecR_wa' NecR_ya' y H.
+rename a' into w.
+
+
+assert (TC7': tc_fn_return Delta' ret retsig).
+{
+  clear - TC7 TS.
+  hnf in TC7|-*. destruct ret; auto.
+  destruct ((temp_types Delta) ! i) eqn:?; try contradiction.
+  destruct TS.
+  specialize (H i); rewrite Heqo in H. subst t.
+  destruct ((temp_types Delta') ! i ).
+  destruct H; auto.
+  auto.
+} (*clear TC7.*)
+rewrite !later_andp in H0.
+apply extend_sepcon_andp in H0; auto.
+destruct H0 as [[TC1 TC2] pre].
+
+normalize in pre. unfold func_ptr_early in *.
+destruct pre as [z1 [z2 [JZ [HF0 pre]]]].
+destruct pre as [[b [EvalA funcatb]] HP].
+destruct (level w) eqn: Hl.
+{ apply own.bupd_intro; repeat intro.
+  rewrite Hl; constructor. }
+rewrite <- Hl in *.
+destruct (levelS_age w n) as (w' & Hage & Hw'); auto.
+
+destruct funcatb as [gs [GS funcatb]]; simpl in GS.
+assert (funcatb_w: (func_at gs (b, 0)) w). 
+{ clear - JZ funcatb. specialize (corable_func_at gs (b,0)); intros. 
+  forget (func_at gs (b,0)) as P. rewrite corable_spec in H. 
+  apply (H z2); trivial. apply join_comm in JZ. eapply join_core. apply JZ. }
+unfold func_at, pureat in funcatb_w. 
+
+assert (Hpsi: filter_genv psi = ge_of (construct_rho (filter_genv psi) vx tx)) by reflexivity.
+unfold filter_genv in Hpsi.
+remember (construct_rho (filter_genv psi) vx tx) as rho.
+set (args := eval_exprlist (snd (split argsig)) bl rho).
+
+(*Here
+specialize (funassertDelta (b) (mk_funspec (argsig,retsig) cc A P Q NEP NEQ) _ (necR_refl _)).
+spec H7.
+1: apply func_at_func_at'; apply H6.*)
+
+assert (MYPROP: exists id fs, Map.get (ge_of rho) id = Some b /\ 
+         (glob_specs Delta') ! id = Some fs /\ func_at fs (b, 0) w).
+{ clear - funcatb_w funassertDelta' GS.
+  assert (XX: exists id:ident, (Map.get (ge_of rho) id = Some b)
+                               /\ exists fs, (glob_specs Delta')!id = Some fs).
+  { destruct funassertDelta' as [_ FD]. 
+    apply (FD b (argsig, retsig) cc _ (necR_refl _)); clear FD.
+    simpl. destruct gs. hnf in funcatb_w. destruct GS as [[? ?] _]; subst. (* destruct GS as [? [? ?]]; subst.*)
+    eexists. eapply funcatb_w. }
+  destruct XX as [id [Hb [fs specID]]]; simpl in Hb.
+
+  assert (exists v, Map.get (ge_of rho) id = Some v /\ func_at fs (v, 0) w).
+  { destruct funassertDelta' as [funassertDeltaA _].
+    destruct (funassertDeltaA id fs _ (necR_refl _) specID) as [v [Hv funcatv]]; simpl in Hv.
+    exists v; split; trivial. }
+  destruct H as [v [Hv funcatv]].
+  assert (VB: b=v); [inversion2 Hb Hv; trivial | subst; clear Hb].
+  exists id, fs; auto. }
+destruct MYPROP as [id [fs [RhoID [SpecOfID funcatv]]]].
+destruct fs as [fsig' cc' A' P' Q' NEP' NEQ'].
+unfold func_at in funcatv, funcatb_w. destruct gs.
+hnf in funcatb_w, funcatv. inversion2 funcatv funcatb_w.
+assert (PREPOST: (forall ts x vl, (! |> (P' ts x vl <=> P0 ts x vl)) w) /\
+                 (forall ts x vl, (! |> (Q' ts x vl <=> Q0 ts x vl)) w)).
+{ apply inj_pair2 in H3; 
+  apply (function_pointer_aux); trivial. f_equal; apply H3. }
+clear H3; destruct PREPOST as [Hpre Hpost]. 
+
+fold args in HP. clear Hpsi. remember (construct_rho (filter_genv psi) vx tx) as rho.
+
+assert (typecheck_environ Delta rho) as TC4.
+{ clear - TC3 TS.
+  destruct TC3 as [TC3 TC4].
+  eapply typecheck_environ_sub in TC3; [| eauto].
+  auto.
+} 
+eapply later_derives in TC2; [|apply (tc_exprlist_sub _ _ _ TS); auto].
+eapply later_derives in TC1; [|apply (tc_expr_sub _ _ _ TS); auto].
+clear TC4.
+
+assert (TCD': tc_environ Delta' rho) by eapply TC3.
+
+assert (TCARGS: tc_environ (funsig_tycontext (argsig, retsig)) (make_args (map fst argsig) args rho)).
+{ assert (LaterW': laterR w w'). constructor; trivial.
+  specialize (TC2 _ LaterW'). subst args.
+  apply (tc_environ_make_args' argsig retsig bl rho Delta' TCD' _ TC2).  }
+
+clear Heqrho.
+destruct GS as [[? ?] GS] (* destruct GS as [? [? GS]]*); subst fsig' cc'.
+
+(*rewrite later_sepcon, <- sepcon_assoc in HP.*)
+
+assert (HPP: (|> (F0 rho * F rho * P ts x (make_args (map fst argsig) args rho)))%pred w).
+{ clear - HF0 HP JZ. rewrite sepcon_assoc, later_sepcon. apply now_later in HF0.
+  exists z1, z2;  auto. } clear HP.
+rewrite later_sepcon in HPP.
+destruct HPP as [w1 [w2 [J [W1 W2]]]]; destruct (join_level _ _ _ J) as [LevW1 LevW2].
+destruct (age1_join2 _ J Hage) as [w1' [w2' [J' [Age1 Age2]]]]; destruct (join_level _ _ _ J') as [Lw1' Lw2'].
+
+assert (LA2: laterM w2 w2'). { constructor; trivial. }
+(*specialize (Hpre ts).*)
+specialize (GS ts). hnf in GS.
+fold (@dependent_type_functor_rec ts) in *.
+specialize (W2 _ LA2). 
+
+specialize (GS x (make_args (map fst argsig) args rho)). hnf in GS.
+assert (LW2': (level w >= level w2')%nat). { apply age_level in Age2. destruct (join_level _ _ _ J); omega. }
+destruct (join_level _ _ _ JZ) as [Lev_z1 Lev_z2].
+
+destruct GS as [ts1 [x1 [G TSX1]]]. hnf in TSX1. rewrite Lev_z2 in TSX1.
+destruct (TSX1 _ LW2' _ (necR_refl _)) as [AA BB].
+{ split; trivial. }
+
+specialize (Hpre ts1 x1 (make_args (map fst argsig) args rho)).
+fold (@dependent_type_functor_rec ts1) in *.
+rewrite <- later_unfash in Hpre.
+specialize (Hpre _ (age_laterR Hage)).
+
+
+destruct AA as [u1 [u2 [JU [U1 U2]]]]; destruct (join_level _ _ _ JU) as [Lu1 Lu2].
+hnf in Hpre. destruct (Hpre u2) as [_ HP']; clear Hpre. omega. specialize (HP' _ (necR_refl _) U2).
+
+assert (ArgsW: app_pred (|> (F0 rho * (F rho * G) * P' ts1 x1 (make_args (map (@fst  _ _) argsig)
+  (eval_exprlist (snd (split argsig)) bl rho) rho) )) w).
+{ clear Hpost funcatv SpecOfID Prog_OK RhoID TC7' RGUARD.
+  assert (XX: (|> (F0 rho * F rho * G * P' ts1 x1 (make_args (map (@fst  _ _) argsig)
+     (eval_exprlist (snd (split argsig)) bl rho) rho) )) w). 
+  { rewrite sepcon_assoc. rewrite sepcon_assoc. rewrite <- sepcon_assoc.
+    rewrite later_sepcon.
+    exists w1, w2; split. trivial. split. trivial. hnf; intros. specialize (age_later_nec _ _ _ Age2 H). intros.
+    destruct (nec_join2  JU H0) as [a1' [a2' [JA [A1 A2]]]]; destruct (join_level _ _ _ JA) as [La1 La2].
+    exists a1', a2'; split. trivial. split.
+    + destruct (nec_refl_or_later _ _ A1); subst. trivial. eapply now_later. apply U1. trivial. 
+    + destruct (nec_refl_or_later _ _ A2); subst. trivial. eapply now_later. apply HP'. trivial. }
+  clear - XX. rewrite 2 sepcon_assoc. rewrite 2 sepcon_assoc in XX.
+  intros u U. destruct (XX _ U) as [u1 [u2 [J [U1 U2]]]]; clear XX.
+  exists u1, u2; split; trivial. split; trivial. 
+}
+apply now_later in  RGUARD.
+apply own.bupd_intro; repeat intro; subst.
+eapply semax_call_aux with (F := fun rho => F rho * G)(P:=P')(F0:=F0)(rho:=construct_rho (filter_genv psi) vx tx)
+ (ts:=ts1)(x:=x1)(fsig0:=(argsig, retsig));  try eassumption; try trivial.
+
+simpl RA_normal; auto. clear ArgsW Hpost RGUARD ora. 
+(*assert ((ALL rho' : environ , |>
+ ! ((EX old : val,
+     substopt ret old (fun rho : environ => F rho * G) rho' * maybe_retval (Q0 ts1 x1) (snd (argsig, retsig)) ret rho') >=>
+    (EX old : val, substopt ret old F rho' * maybe_retval (Q ts x) retsig ret rho'))) (m_phi jm)).
+{*) intros rho' l L y Y z YZ [v Z]. exists v.
+assert (TRIV: (forall rho, typecheck_temp_environ rho (PTree.empty type)) /\
+              (typecheck_var_environ (Map.empty (block * type)) (PTree.empty type)) /\ 
+              (forall rho, typecheck_glob_environ rho (PTree.empty type))).
+{ clear. split.
+  { intros; hnf; intros. rewrite PTree.gempty in H; congruence. } split. 
+  { intros; hnf; intros. split; intros. rewrite PTree.gempty in H; congruence. 
+    destruct H. unfold Map.empty, Map.get in H; congruence. } 
+  { intros; hnf; intros. rewrite PTree.gempty in H; congruence. } }
+assert (LEV2': (level w2' >= level w2')%nat) by omega. 
+assert (LEVz: (level w2' >= level z)%nat). 
+{ rewrite Lw2'. apply necR_level in YZ.
+  destruct (age_later Hage L).
+  + subst l; omega. + apply laterR_level in H; omega. }
+destruct ret; simpl.
++ destruct Z as [zz1 [zz2 [JZZ [Z1 Z2]]]]; destruct (join_level _ _ _ JZ) as [Levz1 Levz2]. simpl in Z1, Z2.
+  destruct Z1 as [z1_1 [z1_2 [JZ1 [Z11 Z12]]]]; destruct (join_level _ _ _ JZ1) as [Levz11 Levz12].
+  destruct (join_assoc JZ1 JZZ) as [y11 [JY1 JY2]]; destruct (join_level _ _ _ JY2) as [_ Levy11].
+  assert (LL: (level w2' >= level y11)%nat) by omega. 
+  exists z1_1, y11; split; trivial. split; trivial.
+  apply (BB (get_result1 i rho') _ LL _ (necR_refl _)).
+  simpl; split. { hnf; simpl; intuition. }
+  exists z1_2, zz2; auto.
++ destruct Z as [zz1 [zz2 [JZZ [Z1 Z2]]]]; destruct (join_level _ _ _ JZ) as [Levz1 Levz2]. simpl in Z1, Z2.
+  destruct Z1 as [z1_1 [z1_2 [JZ1 [Z11 Z12]]]]; destruct (join_level _ _ _ JZ1) as [Levz11 Levz12].
+  destruct (join_assoc JZ1 JZZ) as [y11 [JY1 JY2]]; destruct (join_level _ _ _ JY2) as [_ Levy11].
+  assert (LL: (level w2' >= level y11)%nat) by omega. 
+  exists z1_1, y11; split; trivial. split; trivial. 
+  destruct (type_eq retsig Tvoid).
+  - subst retsig. 
+    apply (BB (globals_only rho') _ LL _ (necR_refl _)).
+    simpl; split. hnf; simpl; intuition.
+    exists z1_2, zz2; auto.
+  - assert (Z22: ((fun rho : environ => EX v : val, Q0 ts1 x1 (env_set (globals_only rho) ret_temp v)) rho') zz2).
+    destruct retsig; trivial.  congruence.
+    clear Z2; destruct Z22 as [vv Z2]. 
+    specialize (BB (env_set (globals_only rho') ret_temp vv) _ LL _ (necR_refl _)); spec BB.
+    * simpl; split. hnf; simpl; intuition.
+      exists z1_2, zz2; auto.
+    *  destruct retsig; try solve [ congruence]; exists vv; trivial.
 Qed.
 
 Lemma semax_call_alt:
