veric/semax_conseq.v
@@ -409,7 +409,7 @@ Qed.
 
 Lemma _guard_allp_fun_id:
   forall {Espec: OracleKind} ge Delta' Delta (F P: environ -> pred rmap) f k,
-    tycontext_subsume Delta Delta' ->
+    tycontext_sub Delta Delta' ->
     _guard Espec ge Delta' (fun rho => F rho * P rho) f k = _guard Espec ge Delta' (fun rho => F rho * (allp_fun_id Delta rho && P rho)) f k.
 Proof.
   intros.
@@ -424,11 +424,12 @@ Proof.
   rewrite (andp_comm (allp_fun_id _ _ )), andp_assoc.
   f_equal.
   apply pred_ext; [apply andp_right; auto | apply andp_left2; auto].
-  apply funassert_allp_fun_id_sub; auto.
+  intros w W. hnf.
+  eapply funassert_allp_fun_id_sub; eauto.
 Qed.
 
 Lemma guard_allp_fun_id: forall {Espec: OracleKind} ge Delta' Delta (F P: environ -> pred rmap) k,
-  tycontext_subsume Delta Delta' ->
+  tycontext_sub Delta Delta' ->
   guard Espec ge Delta' (fun rho => F rho * P rho) k = guard Espec ge Delta' (fun rho => F rho * (allp_fun_id Delta rho && P rho)) k.
 Proof.
   intros.
@@ -436,7 +437,7 @@ Proof.
 Qed.
 
 Lemma rguard_allp_fun_id: forall {Espec: OracleKind} ge Delta' Delta (F: environ -> pred rmap) P k,
-  tycontext_subsume Delta Delta' ->
+  tycontext_sub Delta Delta' ->
   rguard Espec ge Delta' (frame_ret_assert P F) k = rguard Espec ge Delta' (frame_ret_assert (conj_ret_assert P (allp_fun_id Delta)) F) k.
 Proof.
   intros.
@@ -446,11 +447,11 @@ Proof.
   rewrite !proj_frame.
   rewrite proj_conj.
   apply _guard_allp_fun_id; auto.
-Qed.
+Qed. 
 
 Lemma _guard_tc_environ:
   forall {Espec: OracleKind} ge Delta' Delta (F P: environ -> pred rmap) f k,
-    tycontext_subsume Delta Delta' ->
+    tycontext_sub Delta Delta' ->
     _guard Espec ge Delta' (fun rho => F rho * P rho) f k = _guard Espec ge Delta' (fun rho => F rho * (!! typecheck_environ Delta rho && P rho)) f k.
 Proof.
   intros.
@@ -470,7 +471,7 @@ Proof.
 Qed.
 
 Lemma guard_tc_environ: forall {Espec: OracleKind} ge Delta' Delta (F P: environ -> pred rmap) k,
-  tycontext_subsume Delta Delta' ->
+  tycontext_sub Delta Delta' ->
   guard Espec ge Delta' (fun rho => F rho * P rho) k = guard Espec ge Delta' (fun rho => F rho * (!! typecheck_environ Delta rho && P rho)) k.
 Proof.
   intros.
@@ -478,7 +479,7 @@ Proof.
 Qed.
 
 Lemma rguard_tc_environ: forall {Espec: OracleKind} ge Delta' Delta (F: environ -> pred rmap) P k,
-  tycontext_subsume Delta Delta' ->
+  tycontext_sub Delta Delta' ->
   rguard Espec ge Delta' (frame_ret_assert P F) k = rguard Espec ge Delta' (frame_ret_assert (conj_ret_assert P (fun rho => !! typecheck_environ Delta rho)) F) k.
 Proof.
   intros.
@@ -516,7 +517,7 @@ Proof.
   apply allp_derives; intros f.
   apply imp_derives; [apply andp_derives; auto |].
   + erewrite (rguard_allp_fun_id _ _ _ _ R') by eauto.
-    erewrite (rguard_tc_environ _ _ _ _ (conj_ret_assert _ _)) by eauto.
+    erewrite (rguard_tc_environ _ _ _ _ (conj_ret_assert R' _)) by eauto.
     rewrite (rguard_except_0 _ _ _ R).
     rewrite (rguard_bupd _ _ _ (except_0_ret_assert _)).
     apply rguard_mono.
